using sepapps in onesize_malloc requires purifying sepapps

bedrock2/src/bedrock2/SepLib.v
@@ -118,17 +118,16 @@ Proof. unfold purify. intros. constructor. Qed.
 
 
 Definition anybytes{width}{BW: Bitwidth width}{word: word width}{mem: map.map word Byte.byte}
-  (sz: Z)(a: word): mem -> Prop := Memory.anybytes a sz.
+  (sz: Z)(a: word)(m: mem): Prop := 0 <= sz /\ Memory.anybytes a sz m.
 
 #[export] Hint Extern 1 (PredicateSize (anybytes ?sz)) => exact sz
 : typeclass_instances.
 
 Lemma purify_anybytes{width}{BW: Bitwidth width}{word: word width}
   {mem: map.map word Byte.byte} sz a:
-  purify (anybytes sz a) True.
+  purify (anybytes sz a) (0 <= sz).
   (* Note:
-     - (0 <= sz) is not enforced right now by Memory.anybytes
      - (sz <= 2^width) would hold (because of max memory size)
      - (sz < 2^width) would be more useful but is not provable currently *)
-Proof. unfold purify. intros. constructor. Qed.
+Proof. unfold purify, anybytes. intros * [? ?]. assumption. Qed.
 #[export] Hint Resolve purify_anybytes : purify.
